mergesort

Leanplay/Basic.lean
@@ -1,1 +1,264 @@
+-- open Mathlib
+import Mathlib.Tactic.Ring
 def hello := "world"
+
+def myMin (a : Nat) (b : Nat) := if a < b then a else b
+
+theorem test (p q : Prop) (hp : p) (hq : q) : p ∧ q ∧ p := by
+  apply And.intro
+  exact hp
+  apply And.intro
+  exact hq
+  exact hp
+
+def split (xs : List Nat) : List Nat × List Nat := (xs.take (xs.length.div 2), xs.drop (xs.length.div 2))
+theorem split_shortens_left : (x y : Nat) -> (rest : List Nat) -> (split (x::y::rest)).fst.length < (x::y::rest).length := by
+  intro x y rest
+  unfold split; simp
+  . unfold Nat.div
+    simp
+    calc
+      rest.length.div 2 ≤ rest.length := by apply Nat.div_le_self
+      rest.length < rest.length + 1 := by rw [Nat.lt_succ]
+theorem split_shortens_right : (x y : Nat) -> (rest : List Nat) -> (split (x::y::rest)).snd.length < (x::y::rest).length := by
+  intro x y rest
+  simp [split]
+  unfold Nat.div
+  split
+  . apply Nat.zero_lt_succ
+  . rename_i h
+    apply absurd h
+    simp
+
+
+theorem eq_append_split (xs : List Nat) : xs = let (a,b) := split xs; a++b := by
+  simp [split]
+
+def merge_sorted : (acc xs ys : List Nat) -> List Nat
+| acc, [], ys => acc ++ ys
+| acc, xs, [] => acc ++ xs
+| acc, x::xs, y::ys =>
+  if x <= y then merge_sorted (acc ++ [x]) xs (y::ys )
+  else merge_sorted (acc ++ [y]) (x::xs) (ys)
+
+theorem pairwise_cons_repeat (x : Nat) (xs : List Nat) (h : (x::xs).Pairwise LE.le) : (x::x::xs).Pairwise LE.le := by
+  rw [List.pairwise_cons]
+  apply And.intro
+  . intro a a_in_xxs
+    rw [List.pairwise_cons] at h
+    rw [List.mem_cons] at a_in_xxs
+    apply Or.elim a_in_xxs
+    . intro a_eq_x; simp [a_eq_x]
+    . intro h2; apply h.left; exact h2
+  . exact h
+
+theorem merge_sorted_sorted_perm :
+  ∀ (total acc xs ys: List Nat),
+  total.Perm (acc ++ xs ++ ys) ->
+  total.Perm (merge_sorted acc xs ys)
+  := by
+  let rec aux :
+    (total acc xs ys: List Nat) ->
+    total.Perm (acc ++ xs ++ ys) ->
+    total.Perm (merge_sorted acc xs ys)
+    := by
+    intro total acc xs ys hperm
+    unfold merge_sorted
+    split
+    . rw [List.append_nil] at hperm; exact hperm
+    . rw [List.append_nil] at hperm; exact hperm
+    . have acc_short : acc.length < total.length := by
+        rename_i a b c d e f g
+        calc
+          acc.length ≤ acc.length + (d :: e).length := by apply Nat.le_add_right
+          _ ≤ acc.length + (d :: e).length + (g.length ) := by apply Nat.le_add_right
+          _ < acc.length + (d :: e).length + (g.length + 1) := by
+              conv => lhs; rw [Nat.add_assoc]
+              conv => rhs; rw [Nat.add_assoc]
+              rw [Nat.add_lt_add_iff_left]
+              rw [Nat.add_lt_add_iff_left]
+              simp [Nat.lt_succ]
+          _ = acc.length + (d :: e).length + (f :: g).length := by
+              conv =>
+                rhs
+                rhs
+                rw [List.length_cons]
+          _ = (acc ++ d :: e).length + (f :: g).length := by rw [List.length_append]
+          _ = (acc ++ d :: e ++ f :: g).length := by rw [← List.length_append]
+          _ = total.length := by apply List.Perm.length_eq; apply List.Perm.symm; exact hperm
+      split
+      . rename_i a b c d e
+        have permshuffle : total.Perm ((acc ++ [a]) ++ b ++ (c :: d)) := by
+          conv =>
+            rhs
+            lhs
+            rw [List.append_assoc]
+            rw [List.singleton_append]
+          exact hperm
+        have : total.length - (acc.length + 1) < total.length - acc.length := by
+          apply Nat.sub_lt_sub_left
+          exact acc_short
+          simp [Nat.lt_succ]
+        exact aux total (acc ++ [a]) b (c :: d) permshuffle
+      . rename_i a bs c ds e
+        have permshuffle1 : (acc ++ a :: bs ++ c :: ds).Perm ((acc ++ [c]) ++ (a :: bs) ++ ds) := by
+          rw [List.perm_iff_count]
+          intro q
+          simp [List.count_append, List.count_cons]
+          split; all_goals split; all_goals ring_nf
+        have permshuffle : total.Perm ((acc ++ [c]) ++ (a :: bs) ++ds) := by
+          apply List.Perm.trans hperm permshuffle1
+        have : total.length - (acc.length + 1) < total.length - acc.length := by
+          apply Nat.sub_lt_sub_left
+          exact acc_short
+          simp [Nat.lt_succ]
+        exact aux total (acc ++ [c]) (a :: bs) ds permshuffle
+    termination_by total.length - acc.length
+
+  intro total acc xs ys hperm
+  exact aux total acc xs ys hperm
+
+theorem merge_sorted_sorted : ∀ (xs ys acc: List Nat),
+    (acc ++ xs).Pairwise LE.le ->
+    (acc ++ ys).Pairwise LE.le ->
+    (merge_sorted acc xs ys).Pairwise LE.le
+    := by
+  intro xs
+  induction xs with
+  | nil =>
+      simp [merge_sorted]
+  | cons x xs ihx =>
+      intro ys
+      induction ys with
+      | nil =>
+          simp [merge_sorted]
+          intro _ axxs_sorted _
+          exact axxs_sorted
+      | cons y ys ihy =>
+          intro acc axxs_sorted ayys_sorted
+          have acc_sorted : List.Pairwise LE.le acc := by
+            apply List.Pairwise.sublist (List.sublist_append_left acc (x::xs))
+            exact axxs_sorted
+          have xxs_sorted : (x :: xs).Pairwise LE.le := by
+            apply List.Pairwise.sublist (List.sublist_append_right acc (x::xs))
+            exact axxs_sorted
+          have yys_sorted : (y :: ys).Pairwise LE.le := by
+            apply List.Pairwise.sublist (List.sublist_append_right acc (y::ys))
+            exact ayys_sorted
+          have xs_sorted : xs.Pairwise LE.le := by apply List.Pairwise.of_cons xxs_sorted
+          have ys_sorted : ys.Pairwise LE.le := by apply List.Pairwise.of_cons yys_sorted
+
+          have acc_all_le_xs : ∀ (a : Nat), a ∈ acc → ∀ (b : Nat), b ∈ x::xs → a ≤ b := by
+            rw [List.pairwise_append] at axxs_sorted
+            exact (And.right (And.right axxs_sorted))
+          have acc_all_le_ys : ∀ (a : Nat), a ∈ acc → ∀ (b : Nat), b ∈ y::ys → a ≤ b := by
+            rw [List.pairwise_append] at ayys_sorted
+            exact (And.right (And.right ayys_sorted))
+
+          unfold merge_sorted
+          split
+          . rename_i x_le_y
+            have xyys_sorted : List.Pairwise LE.le (x :: y :: ys) := by
+              have y_le_yys : ∀ b : Nat, b ∈ y::ys -> y ≤ b := by
+                apply And.left
+                rw [← List.pairwise_cons]
+                apply pairwise_cons_repeat y ys yys_sorted
+              apply List.Pairwise.cons; any_goals exact yys_sorted
+              intro a a_in_yys
+              calc
+                x ≤ y := by exact x_le_y
+                y ≤ a := by apply y_le_yys; exact a_in_yys
+
+            apply ihx
+            . rw [← List.append_cons]; exact axxs_sorted
+            . rw [← List.append_cons]
+              rw [List.pairwise_append]
+              rw [and_iff_right acc_sorted]
+              rw [and_iff_right xyys_sorted]
+              intro a a_in_acc b b_in_xyys
+
+              calc
+                a ≤ x := by apply acc_all_le_xs; exact a_in_acc; simp
+                x ≤ b := by
+                  by_cases h: x=b
+                  . simp [h]
+                  rw [List.mem_cons] at b_in_xyys
+                  have b_in_yys : b ∈ y :: ys := by
+                    apply Or.elim b_in_xyys
+                    . intro h'; apply absurd (Eq.symm h') h
+                    . simp
+                  have x_le_yys : ∀ c : Nat, c ∈ y :: ys → x ≤ c := by
+                    apply And.left
+                    rw [← List.pairwise_cons]
+                    exact xyys_sorted
+                  apply x_le_yys
+                  exact b_in_yys
+
+          . rename_i nx_le_y
+            have y_le_x : y ≤ x := by apply Nat.le_of_not_le; exact nx_le_y
+            have yxxs_sorted : List.Pairwise LE.le (y :: x :: xs) := by
+              have x_le_xxs : ∀ b : Nat, b ∈ x::xs -> x ≤ b := by
+                apply And.left
+                rw [← List.pairwise_cons]
+                apply pairwise_cons_repeat x xs xxs_sorted
+              apply List.Pairwise.cons; any_goals exact xxs_sorted
+              intro a a_in_xxs
+              calc
+                y ≤ x := by exact y_le_x
+                x ≤ a := by apply x_le_xxs; exact a_in_xxs
+
+            apply ihy
+            . rw [← List.append_cons]
+              rw [List.pairwise_append]
+              rw [and_iff_right acc_sorted]
+              rw [and_iff_right yxxs_sorted]
+              intro a a_in_acc b b_in_yxxs
+
+              calc
+                a ≤ y := by apply acc_all_le_ys; exact a_in_acc; simp
+                y ≤ b := by
+                  by_cases h: y=b
+                  . simp [h]
+                  rw [List.mem_cons] at b_in_yxxs
+                  have b_in_xxs : b ∈ x :: xs := by
+                    apply Or.elim b_in_yxxs
+                    . intro h'; apply absurd (Eq.symm h') h
+                    . simp
+                  have y_le_xxs : ∀ c : Nat, c ∈ x :: xs → y ≤ c := by
+                    apply And.left
+                    rw [← List.pairwise_cons]
+                    exact yxxs_sorted
+                  apply y_le_xxs
+                  exact b_in_xxs
+            . rw [← List.append_cons]; exact ayys_sorted
+
+
+
+def mergesort : (xs : List Nat) -> List Nat
+| [] => []
+| [x] => [x]
+| x::y::rest =>
+  let left := (split (x::y::rest)).fst
+  let right := (split (x::y::rest)).snd
+  merge_sorted [] (mergesort left) (mergesort right)
+termination_by xs => xs.length
+decreasing_by
+  apply split_shortens_left
+  apply split_shortens_right
+
+theorem mergesort_sorted : ∀ (xs : List Nat), (mergesort xs).Pairwise LE.le
+| [] => by simp [mergesort]
+| [x] => by simp [mergesort]
+| x::y::rest => by
+    unfold mergesort
+    apply merge_sorted_sorted
+    . simp
+      apply mergesort_sorted
+    . simp
+      apply mergesort_sorted
+termination_by xs => xs.length
+decreasing_by
+  apply split_shortens_left
+  apply split_shortens_right
+
+#eval mergesort [5, 2, 0, 1, 1, 7, 7, 1, 2, 0, 1, 9, 7, 8, 4, 1, 8, 0, 6, 3, 3, 3, 9, 5, 7, 3, 8, 1, 8, 1, 8, 3, 5, 5, 1, 1, 9, 7, 8, 4, 4, 6, 5, 2, 1, 0, 2, 5, 0, 1, 0, 3, 8, 2, 9, 7, 7, 6, 2, 5, 0, 0, 9, 4, 1, 0, 2, 2, 6, 7, 2, 3, 7, 6, 7, 3, 7, 4, 5, 1, 8, 3, 4, 4, 1, 2, 6, 6, 1, 4, 8, 2, 5, 6, 3, 6, 0, 4, 7, 7]
